Hmm...

LogicalRefinement/Denot/Subst.lean
@@ -10,12 +10,28 @@ def ValidSubst {Γ Δ: Context}
   (I: Stlc.InterpSubst Γ.upgrade.stlc Δ.upgrade.stlc): Prop 
   := ∀G, (G ⊧ ✓Γ) -> (I.transport_ctx G ⊧ ✓Δ)
 
+abbrev SubstCtx.interp_up {σ Γ Δ} (S: SubstCtx σ Γ Δ) (IΔ: IsCtx Δ)
+  : Stlc.InterpSubst Γ.upgrade.stlc Δ.upgrade.stlc
+  := Stlc.SubstCtx.interp (SubstCtx.stlc S.upgrade IΔ.upgrade)
+
+abbrev SubstCtx.transport_interp_up {σ Γ Δ}
+  (S: SubstCtx σ Γ Δ)
+  (IΔ: IsCtx Δ)
+  (G: Γ.upgrade.stlc.interp)
+  : Δ.upgrade.stlc.interp
+  := Stlc.InterpSubst.transport_ctx (S.interp_up IΔ) G
+
 theorem Term.denote_ty.subst {Γ Δ: Context} {σ} {G: Γ.upgrade.stlc.interp} {A: Term} {a}
-  (H: A.denote_ty Γ.upgrade.sparsity G a)
+  (Ha: A.denote_ty Γ.upgrade.sparsity G a)
   (S: SubstCtx σ Γ Δ)
   (IΓ: IsCtx Γ) (IΔ: IsCtx Δ)
-  (V: ValidSubst (Stlc.SubstCtx.interp (SubstCtx.stlc S.upgrade IΔ.upgrade)))
-  : True
+  (HG: G ⊧ ✓Γ)
+  (V: ValidSubst (S.interp_up IΔ))
+  (HA: Γ ⊢ A: sort s)
+  : (A.subst σ).denote_ty 
+    Δ.upgrade.sparsity 
+    (S.transport_interp_up IΔ G) 
+    (HA.stlc_ty_subst ▸ a)
   := by sorry
 
 theorem HasType.denote_subst0'
